# 780. Reaching Points

## Tag

- Math
- Goldman Sachs

## Description

Given four integers `sx`, `sy`, `tx`, and `ty`, return `true` *if it is possible to convert the point* `(sx, sy)` *to the point* `(tx, ty)` *through some operations**, or* `false` *otherwise*.

The allowed operation on some point `(x, y)` is to convert it to either `(x, x + y)` or `(x + y, y)`.

 

**Example 1:**

```
Input: sx = 1, sy = 1, tx = 3, ty = 5
Output: true
Explanation:
One series of moves that transforms the starting point to the target is:
(1, 1) -> (1, 2)
(1, 2) -> (3, 2)
(3, 2) -> (3, 5)
```

**Example 2:**

```
Input: sx = 1, sy = 1, tx = 2, ty = 2
Output: false
```

**Example 3:**

```
Input: sx = 1, sy = 1, tx = 1, ty = 1
Output: true
```

 

**Constraints:**

- `1 <= sx, sy, tx, ty <= 109`



## Solution

> Work backwards + use modulo operation

- If we solve this problem in the start -> end order, there are 2 possible next step, however for backwards there is onle ONE parent
- For optimization, we bundle the possible solution together for as long as `tx > ty` or `ty>tx`

```java
class Solution {
    public boolean reachingPoints(int sx, int sy, int tx, int ty) {
        // Idea: reverse direction, reach start from end
        // Corner case
        if (tx < sx || ty < sy) {
            return false;
        }
        
        while (tx >= sx && ty >= sy) {
            if (tx == ty) {
                // Case 1: can't move any more
                break;
            } else if (tx > ty) {
                // Case 2: decrease x
                if (ty > sy) {
                    tx %= ty;
                } else {
                    // already ty == sy
                    return (tx - sx) % ty == 0;
                }
            } else {
                // Case 3: decrease y
                if (tx > sx) {
                    ty %= tx;
                } else {
                    // already tx == sx
                    return (ty - sy) % tx == 0;
                }
            }
        }

        return tx == sx && ty == sy;
    }
}
```

 **TC: O(log(max(tx, ty)))**

**SC: O(1)**

*for unoptimized solution, the TC is O(max(tx, ty))*